specs/experimental/Spec.Seq.Lib.fst
@@ -1,0 +1,57 @@
+module Spec.Seq.Lib
+
+open FStar.Seq
+open FStar.Mul
+open FStar.UInt
+
+module U8 = FStar.UInt8
+module U32 = FStar.UInt32
+open U32
+
+type seq 'a = s:Seq.seq 'a{length s < pow2 32}
+type byte = UInt8.t
+type bytes = seq byte
+type lseq 'a n = s:seq 'a{length s = U32.v n}
+type lbytes n = s:bytes{length s = U32.v n}
+
+val create: #a:Type -> sz:U32.t -> v:a -> s:seq a{length s = U32.v sz}
+let create #a s v = Seq.create #a (U32.v s) v
+
+val upd: #a:Type -> s:seq a -> i:U32.t{U32.v i < length s} -> 
+	 v:a -> s':seq a{length s' = length s}
+let upd #a s i v = Seq.upd #a s (U32.v i) v
+
+val index: #a:Type -> s:seq a -> i:U32.t{U32.v i < length s} -> a
+let index #a s i = Seq.index #a s (U32.v i)
+
+let op_String_Access = index
+let op_String_Assignment = upd
+
+val slice: #a:Type -> s:seq a -> i:U32.t -> j:U32.t{U32.v i <= U32.v j /\ U32.v j <= length s} -> t:seq a {length t = U32.v j - U32.v i}
+let slice #a s i j = Seq.slice #a s (U32.v i) (U32.v j)
+
+val seq_length: #a:Type -> s:seq a -> r:U32.t{U32.v r = length s}
+let seq_length (#a:Type) (s:seq a) = U32.uint_to_t (length s)
+
+val blit: #a:Type ->
+	s1:seq a -> ind_s1:U32.t{U32.v ind_s1 <= length s1} ->
+	s2:seq a -> ind_s2:U32.t{U32.v ind_s2 <= length s2} ->
+	len:U32.t{U32.v ind_s1 + U32.v len <= length s1 /\ 
+		  U32.v ind_s2 + U32.v len <= length s2} ->
+	Tot (res:seq a{length res = length s2}) 
+
+#reset-options "--z3rlimit 30"
+
+let blit #a s1 ind_s1 s2 ind_s2 len =
+    let t1 = slice s2 0ul ind_s2 in
+    let t3 = slice s2 (ind_s2 +^ len) (seq_length s2)  in
+    let f2 = slice s1 ind_s1 (ind_s1 +^ len)  in
+    t1 @| f2 @| t3
+
+val update_slice: #a:Type -> s:seq a -> i:U32.t -> l:U32.t{U32.v i + U32.v l <= length s} -> 
+		  f: (s:lseq a l -> s:lseq a l) -> Tot (r:seq a{length r = length s})
+let update_slice #a s i l f = 
+    let s1 = slice s 0ul i in
+    let s2 = slice s i (i +^ l) in
+    let s3 = slice s (i +^ l) (seq_length s) in
+    s1 @| (f s2) @| s3
